theories/queue_lib.v
@@ -1,6 +1,7 @@
-From stdpp               Require Import list.
-From iris.program_logic  Require Import weakestpre.
-From hazel               Require Import notation weakestpre.
+From stdpp              Require Import list.
+From iris.proofmode     Require Import base tactics classes.
+From iris.program_logic Require Import weakestpre.
+From hazel              Require Import notation weakestpre list_lib heap.
 
 Class QueueLib Σ `{!irisG eff_lang Σ} := {
   queue_create : val;
@@ -17,7 +18,7 @@ Class QueueLib Σ `{!irisG eff_lang Σ} := {
   queue_create_spec E :
     ⊢ EWP queue_create #() @ E {{ q, ∀ I, is_queue q I 0%nat }};
 
-  queue_push_spec E q I n v :
+  queue_push_spec E q I (n : nat) v :
     ▷ is_queue q I n -∗
       ▷ I v -∗
         EWP queue_push q v @ E {{ _, is_queue q I (S n) }};
@@ -41,3 +42,125 @@ Global Instance is_queue_proper `{QueueLib} q :
 Proof.
   intros ??????. apply equiv_dist=>n. apply is_queue_ne; by apply equiv_dist.
 Qed.
+
+
+Section QueueLibModel.
+Context `{!heapG Σ}.
+
+Definition is_queue' : val -d> (val -d> iPropO Σ) -d> natO -d> iPropO Σ := λ q I n,
+  (∃ l us, ⌜ q = #(l : loc) ⌝ ∗ l ↦ (list_encoding' us) ∗
+           ⌜ length us = n  ⌝ ∗ [∗ list] u ∈ us, I u)%I.
+Instance is_queue_ne' q n : Proper ((dist n) ==> (dist n) ==> (dist n)) (is_queue' q).
+Proof. solve_proper. Qed.
+
+Definition queue_create' : val := λ: <>, ref (list_encoding' []).
+Definition queue_push'   : val := λ: "q" "v", "q" <- (list_cons' "v" (Load "q")).
+Definition queue_pop'    : val := λ: "q",
+  match: (Load "q") with InjL <>  => #() | InjR "p" => "q" <- (Snd "p");; Fst "p" end.
+Definition queue_empty'  : val := λ: "q",
+  match: (Load "q") with InjL <>  => #true | InjR <> => #false end.
+
+Lemma queue_create_spec' E :
+  ⊢ EWP queue_create' #() @ E {{ q, ∀ I, is_queue' q I 0%nat }}.
+Proof.
+  iApply ewp_pure_step. apply pure_prim_step_beta. simpl.
+  iApply ewp_mono'. { by iApply ewp_alloc. }
+  iIntros (q) "H". iDestruct "H" as (l) "[-> Hl]".
+  iModIntro. iIntros (I). iExists l, []. by eauto with iFrame.
+Qed.
+
+Lemma queue_push_spec' E q I (n : nat) v :
+  ▷ is_queue' q I n -∗
+    ▷ I v -∗
+      EWP queue_push' q v @ E {{ _, is_queue' q I (S n) }}.
+Proof.
+  iIntros "Hq HI".
+  iApply (Ectxi_ewp_bind (AppLCtx _)). done.
+  iApply ewp_pure_step'. apply pure_prim_step_beta. simpl.
+  iApply ewp_pure_step.  apply pure_prim_step_rec.
+  iApply ewp_value.
+  iApply ewp_pure_step.  apply pure_prim_step_beta. simpl.
+  iNext. iDestruct "Hq" as (l us) "(-> & Hl & % & Hinv)".
+  iApply (Ectxi_ewp_bind (StoreRCtx _)). done.
+  iApply (Ectxi_ewp_bind (AppRCtx _)). done.
+  iApply (ewp_mono' with "[Hl]"). { by iApply (ewp_load with "Hl"). }
+  iIntros (w) "[-> Hl]". iModIntro. simpl.
+  iApply ewp_mono'. { by iApply (list_cons_spec' _ _ _ us). }
+  iIntros (w) "->". iModIntro. simpl.
+  iApply (ewp_mono' with "[Hl]"). { by iApply (ewp_store with "Hl"). }
+  iIntros (_) "Hl". iModIntro. iExists l, (v :: us). iFrame.
+  iPureIntro. split; [done|]. simpl. by rewrite H.
+Qed.
+
+Lemma queue_pop_spec' E q I n :
+  ▷ is_queue' q I (S n) -∗
+    EWP queue_pop' q @ E {{ v, is_queue' q I n ∗ I v }}.
+Proof.
+  iIntros "Hq".
+  iApply ewp_pure_step'. apply pure_prim_step_beta. simpl.
+  iNext. iDestruct "Hq" as (l us) "(-> & Hl & % & Hinv)".
+  case us as [|u us]; [done|]. iDestruct "Hinv" as "[HI Hinv]".
+  iApply (Ectxi_ewp_bind (CaseCtx _ _)). done.
+  iApply (ewp_mono' with "[Hl]"). { by iApply (ewp_load with "Hl"). }
+  iIntros (w) "[-> Hl]". iModIntro. simpl.
+  iApply ewp_pure_step. apply pure_prim_step_case_InjR.
+  iApply (Ectxi_ewp_bind (AppLCtx _)). done.
+  iApply ewp_pure_step. apply pure_prim_step_rec.
+  iApply ewp_value.
+  iApply ewp_pure_step. apply pure_prim_step_beta. simpl.
+  iApply (Ectxi_ewp_bind (AppRCtx   _)). done.
+  iApply (Ectxi_ewp_bind (StoreRCtx _)). done.
+  iApply ewp_pure_step. apply pure_prim_step_Snd.
+  iApply ewp_value. simpl.
+  iApply (ewp_mono' with "[Hl]"). { by iApply (ewp_store with "Hl"). }
+  iIntros (w) "Hl". iModIntro.
+  iApply (Ectxi_ewp_bind (AppLCtx _)). done.
+  iApply ewp_pure_step. apply pure_prim_step_rec. iApply ewp_value.
+  iApply ewp_pure_step. apply pure_prim_step_beta. simpl.
+  iApply ewp_pure_step. apply pure_prim_step_Fst. iApply ewp_value.
+  iFrame. iExists l, us. by eauto with iFrame.
+Qed.
+
+Lemma queue_empty_spec' E q I n :
+  ▷ is_queue' q I n -∗
+    EWP queue_empty' q @ E {{ v, is_queue' q I n ∗
+                             match n with
+                             | 0%nat => ⌜ v = #true  ⌝
+                             | S n   => ⌜ v = #false ⌝
+                             end
+                           }}.
+Proof.
+  iIntros "Hq".
+  iApply ewp_pure_step'. apply pure_prim_step_beta. simpl.
+  iNext. iDestruct "Hq" as (l us) "(-> & Hl & % & Hinv)".
+  iApply (Ectxi_ewp_bind (CaseCtx _ _)). done.
+  iApply (ewp_mono' with "[Hl]"). { by iApply (ewp_load with "Hl"). }
+  iIntros (w) "[-> Hl]". iModIntro. simpl.
+  case us as [|u us].
+  - iApply ewp_pure_step. apply pure_prim_step_case_InjL.
+    iApply (Ectxi_ewp_bind (AppLCtx _)). done.
+    iApply ewp_pure_step. apply pure_prim_step_rec.  iApply ewp_value.
+    iApply ewp_pure_step. apply pure_prim_step_beta. iApply ewp_value.
+    rewrite <-H. simpl. iSplit; [|done]. iExists l, []. by auto.
+  - case n as [|n]; [done|].
+    iApply ewp_pure_step. apply pure_prim_step_case_InjR.
+    iApply (Ectxi_ewp_bind (AppLCtx _)). done.
+    iApply ewp_pure_step. apply pure_prim_step_rec.  iApply ewp_value.
+    iApply ewp_pure_step. apply pure_prim_step_beta. iApply ewp_value.
+    iSplit; [|done]. iExists l, (u :: us). by iFrame.
+Qed.
+
+Program Instance QueueLib_valid : QueueLib Σ := {
+  queue_create      := queue_create';
+  queue_push        := queue_push';
+  queue_pop         := queue_pop';
+  queue_empty       := queue_empty';
+  is_queue          := is_queue';  
+  is_queue_ne       := is_queue_ne';
+  queue_create_spec := queue_create_spec';
+  queue_push_spec   := queue_push_spec';
+  queue_pop_spec    := queue_pop_spec';
+  queue_empty_spec  := queue_empty_spec';
+}.
+
+End QueueLibModel.
