theories/adequacy.v
@@ -1,12 +1,9 @@
 From iris.proofmode      Require Import base tactics classes.
 From iris.base_logic.lib Require Import iprop wsat.
-From iris.program_logic  Require Import weakestpre.
-From hazel               Require Import notation weakestpre.
+From iris.program_logic  Require Import weakestpre adequacy.
+From hazel               Require Import notation weakestpre heap.
 
-Section adequacy.
-Context `{!irisG eff_lang Σ}.
-
-Lemma ewp_imp_wp e Φ :
+Lemma ewp_imp_wp `{!irisG eff_lang Σ} e Φ :
  EWP e <| ⊥ |> {{ v, Φ v }} ⊢ WP e @ NotStuck; ⊤ {{ Φ }}.
 Proof.
   iLöb as "IH" forall (e).
@@ -26,5 +23,45 @@ Proof.
     iModIntro. by iSplitL; [iApply "IH"|].
 Qed.
 
-End adequacy.
+Section adequacy.
+  Context `{!heapPreG Σ}.
 
+  Lemma eff_heap_adequacy s e σ φ :
+    (∀ `{!heapG Σ}, ⊢ WP e @ s; ⊤ {{ v, ⌜φ v⌝ }}) →
+    adequate s e σ (λ v _, φ v).
+  Proof.
+    intros Hwp; eapply (wp_adequacy _ _); iIntros (??) "".
+    iMod (gen_heap_init σ.(heap)) as (?) "Hh".
+    iMod (inv_heap_init loc val) as (?) ">Hi".
+    iModIntro. iExists
+      (λ σ κs, gen_heap_ctx σ.(heap)),
+      (λ _, True%I).
+    iFrame. iApply (Hwp (HeapG _ _ _ _)).
+  Qed.
+
+  Lemma eff_adequacy e σ φ :
+    (∀ `{!heapG Σ}, ⊢ EWP e <| ⊥ |> {{ v, ⌜φ v⌝ }}) →
+    adequate NotStuck e σ (λ v _, φ v).
+  Proof.
+    intros Hwp.
+    apply eff_heap_adequacy.
+    intros.
+    iApply ewp_imp_wp. iApply Hwp.
+  Qed.
+
+  Lemma eff_adequate_not_stuck e σ Φ :
+  (∀ `{!heapG Σ}, ⊢ EWP e <| ⊥ |> {{ Φ }}) →
+  ∀ e' σ', rtc erased_step ([e], σ) ([e'], σ') →
+            not_stuck e' σ'.
+  Proof.
+    intros Hewp ?? Hstep.
+    assert (adequate NotStuck e σ (λ _ _, True)) as Hadequate.
+    { apply eff_adequacy.
+      intros.
+      iApply ewp_mono'; [ iApply Hewp | ].
+      by iIntros (?) "_". }
+    eapply adequate_alt in Hadequate as [_ Hnot_stuck]; eauto.
+    apply Hnot_stuck; auto.
+    set_solver.
+  Qed.
+End adequacy.
